feat: normalize AIGs up to commutativity

LeanSAT/AIG/Cached.lean
@@ -69,45 +69,53 @@ programmming, for proving purposes use `AIG.mkGate` and equality theorems to thi
 Beyond caching this function also implements a subset of the optimizations presented in:
 -/
 def mkGateCached (aig : AIG α) (input : GateInput aig) : Entrypoint α :=
-  let ⟨decls, cache, inv⟩ := aig
   let lhs := input.lhs.ref.gate
   let rhs := input.rhs.ref.gate
-  let linv := input.lhs.inv
-  let rinv := input.rhs.inv
-  have := input.lhs.ref.hgate
-  have := input.rhs.ref.hgate
-  let decl := .gate lhs rhs linv rinv
-  match cache.find? decl with
-  | some hit =>
-    ⟨⟨decls, cache, inv⟩, ⟨hit.idx, hit.hbound⟩⟩
-  | none =>
-    /-
-    Here we implement the constant propagating subset of:
-    https://fmv.jku.at/papers/BrummayerBiere-MEMICS06.pdf
-    TODO: rest of the table
-    -/
-    match decls[lhs], decls[rhs], linv, rinv with
-    -- Boundedness
-    | .const true, _, true, _ | .const false, _, false, _
-    | _, .const true, _, true | _, .const false, _, false =>
-      mkConstCached ⟨decls, cache, inv⟩ false
-    -- Left Neutrality
-    | .const true, _, false, false | .const false, _, true, false =>
-      ⟨⟨decls, cache, inv⟩, rhs, (by assumption)⟩
-    -- Right Neutrality
-    | _, .const true, false, false | _, .const false, false, true =>
-      ⟨⟨decls, cache, inv⟩, lhs, (by assumption)⟩
-    | _, _, _, _ =>
-      let g := decls.size
-      let cache := cache.insert decls decl
-      let decls := decls.push decl
-      have inv := by
-        intro lhs rhs linv rinv i h1 h2
-        simp only [decls] at *
-        simp only [Array.get_push] at h2
-        split at h2
-        . apply inv <;> assumption
-        . injections; omega
-      ⟨⟨decls, cache, inv⟩, ⟨g, by simp [g, decls]⟩⟩
+  if lhs < rhs then
+    go aig ⟨input.lhs, input.rhs⟩
+  else
+    go aig ⟨input.rhs, input.lhs⟩
+where
+  go (aig : AIG α) (input : GateInput aig) : Entrypoint α :=
+    let ⟨decls, cache, inv⟩ := aig
+    let lhs := input.lhs.ref.gate
+    let rhs := input.rhs.ref.gate
+    let linv := input.lhs.inv
+    let rinv := input.rhs.inv
+    have := input.lhs.ref.hgate
+    have := input.rhs.ref.hgate
+    let decl := .gate lhs rhs linv rinv
+    match cache.find? decl with
+    | some hit =>
+      ⟨⟨decls, cache, inv⟩, ⟨hit.idx, hit.hbound⟩⟩
+    | none =>
+      /-
+      Here we implement the constant propagating subset of:
+      https://fmv.jku.at/papers/BrummayerBiere-MEMICS06.pdf
+      TODO: rest of the table
+      -/
+      match decls[lhs], decls[rhs], linv, rinv with
+      -- Boundedness
+      | .const true, _, true, _ | .const false, _, false, _
+      | _, .const true, _, true | _, .const false, _, false =>
+        mkConstCached ⟨decls, cache, inv⟩ false
+      -- Left Neutrality
+      | .const true, _, false, false | .const false, _, true, false =>
+        ⟨⟨decls, cache, inv⟩, rhs, (by assumption)⟩
+      -- Right Neutrality
+      | _, .const true, false, false | _, .const false, false, true =>
+        ⟨⟨decls, cache, inv⟩, lhs, (by assumption)⟩
+      | _, _, _, _ =>
+        let g := decls.size
+        let cache := cache.insert decls decl
+        let decls := decls.push decl
+        have inv := by
+          intro i lhs rhs linv rinv h1 h2
+          simp only [decls] at *
+          simp only [Array.get_push] at h2
+          split at h2
+          . apply inv <;> assumption
+          . injections; omega
+        ⟨⟨decls, cache, inv⟩, ⟨g, by simp [g, decls]⟩⟩
 
 end AIG
